$$\huge
\vec{E}=\vec{E}_{0}\sin(\vec{k}\vec{r}-\omega t)
$$
Mit $\vec{k}=(0,0,k_{z})$ Ã¼ber $rot \vec{E}=-\dot{\vec{B}}$ ergibt $\frac{ \partial E_{x} }{ \partial y }-\frac{ \partial E_{y} }{ \partial z }=-E_{0k_{z}\cos(k_{z}z-\omega t)}$

$$\large
B_{z}(z,t)=-E_{0} \frac{k_{z}}{\omega}\sin(k_{z}z-\omega t)=-\frac{E_{y}(z,t)}{c}
$$
---
$$\huge
\vec{E} \perp \vec{B} \qquad \vec{E},\vec{B}\perp \vec{k}
$$
E und B sind in Phase
$$\huge
\lvert \vec{B} \rvert =\frac{\lvert \vec{E} \rvert }{c}
$$

---
$$\huge
\vec{B}=\frac{1}{\omega}(\vec{k}\times \vec{E}) \qquad \vec{E}=\frac{\omega}{k^2}(\vec{k}\times\vec{B})
$$
---
$$\huge
\lambda=\frac{c}{f}
$$
